pcuic/theories/PCUICSubstitution.v
@@ -356,7 +356,7 @@ Lemma subst_declared_symbol `{checker_flags} :
     declared_symbol Σ k decl ->
     nth_error (symbols decl) n = Some ty ->
     let ty' :=
-      subst0 (symbols_subst k n u #|symbols decl|) (subst_instance_constr u ty)
+      subst0 (symbols_subst k (S n) u #|symbols decl|) (subst_instance_constr u ty)
     in
     subst s i ty' = ty'.
 Proof.
@@ -1196,6 +1196,26 @@ Proof.
   - simpl. constructor.
     now rewrite nth_error_map H.
 
+  - rewrite 2!distr_subst_rec.
+    rewrite (subst_closedn _ _ (PCUICAst.lhs r)).
+    1:{ eapply closed_upwards. 1: eapply closed_rule_lhs.
+        all: eauto.
+        subst ss. rewrite symbols_subst_length. lia.
+    }
+    rewrite (subst_closedn _ _ (PCUICAst.rhs r)).
+    1:{ eapply closed_upwards. 1: eapply closed_rule_rhs.
+        all: eauto.
+        subst ss. rewrite symbols_subst_length. lia.
+    }
+    assert (e : forall s n, map (subst s n) ss = ss).
+    { intros s' n'. subst ss. unfold symbols_subst.
+      rewrite list_make_map. simpl. reflexivity.
+    }
+    rewrite e.
+    replace #|s0| with #|map (subst s #|Γ''|) s0| by (now rewrite map_length).
+    eapply red_rewrite_rule. all: eauto.
+    rewrite map_length. assumption.
+
   - constructor.
     specialize (IHred1 Γ0 Γ' (Γ'' ,, vass na N) eq_refl).
     now rewrite subst_context_snoc0 in IHred1.
@@ -1322,6 +1342,27 @@ Proof.
 
   - simpl. apply red1_red; constructor.
     now rewrite nth_error_map H.
+
+  - rewrite 2!distr_subst_rec.
+    rewrite (subst_closedn _ _ (PCUICAst.lhs r)).
+    1:{ eapply closed_upwards. 1: eapply closed_rule_lhs.
+        all: eauto.
+        subst ss. rewrite symbols_subst_length. lia.
+    }
+    rewrite (subst_closedn _ _ (PCUICAst.rhs r)).
+    1:{ eapply closed_upwards. 1: eapply closed_rule_rhs.
+        all: eauto.
+        subst ss. rewrite symbols_subst_length. lia.
+    }
+    assert (e : forall s n, map (subst s n) ss = ss).
+    { intros s' n'. subst ss. unfold symbols_subst.
+      rewrite list_make_map. simpl. reflexivity.
+    }
+    rewrite e.
+    replace #|s0| with #|map (subst s #|Γ'|) s0| by (now rewrite map_length).
+    econstructor. 1: constructor.
+    eapply red_rewrite_rule. all: eauto.
+    rewrite map_length. assumption.
 
   - specialize (IHred1 Γ0 Δ Γ' eq_refl wfΓ Hs).
     apply red_abs. auto. constructor.
@@ -1487,6 +1528,27 @@ Proof.
 
   - simpl. apply red1_red; constructor.
     now rewrite nth_error_map H.
+
+  - rewrite 2!distr_subst_rec.
+    rewrite (subst_closedn _ _ (PCUICAst.lhs r)).
+    1:{ eapply closed_upwards. 1: eapply closed_rule_lhs.
+        all: eauto.
+        subst ss. rewrite symbols_subst_length. lia.
+    }
+    rewrite (subst_closedn _ _ (PCUICAst.rhs r)).
+    1:{ eapply closed_upwards. 1: eapply closed_rule_rhs.
+        all: eauto.
+        subst ss. rewrite symbols_subst_length. lia.
+    }
+    assert (e : forall s n, map (subst s n) ss = ss).
+    { intros s' n'. subst ss. unfold symbols_subst.
+      rewrite list_make_map. simpl. reflexivity.
+    }
+    rewrite e.
+    replace #|s0| with #|map (subst s #|Γ'|) s0| by (now rewrite map_length).
+    econstructor. 1: constructor.
+    eapply red_rewrite_rule. all: eauto.
+    rewrite map_length. assumption.
 
   - specialize (IHred1 Γ0 Δ Γ' eq_refl Hs).
     apply red_abs. auto. constructor.
