template-coq/theories/EnvironmentTyping.v
@@ -450,12 +450,9 @@ Module DeclarationTyping (T : Term) (E : EnvironmentSig T)
 
     Record on_rewrite_rule Σ (Δ : context) (r : rewrite_rule) := {
       rewCommonType : term ;
-      lhsTyped :
-        P Σ (Δ ,,, r.(pat_context))
-          (mkElims (tRel (#|r.(pat_context)| + r.(head))) r.(elims))
-          (Some rewCommonType) ;
-      rhsTyped : P Σ (Δ ,,, r.(pat_context)) r.(rhs) (Some rewCommonType) ;
-      onHead : r.(head) < #|Δ| ;
+      lhsTyped : P Σ (Δ ,,, r.(pat_context)) (lhs r) (Some rewCommonType) ;
+      rhsTyped : P Σ (Δ ,,, r.(pat_context)) (rhs r) (Some rewCommonType) ;
+      onHead : r.(head) < #|Δ| ; (* TODO Remove? *)
       onElims : Forall (elim_pattern #|r.(pat_context)|) r.(elims)
     }.
 
